working out more semantics.

theories/HoareSemantics.v
@@ -2,16 +2,21 @@ From Coq.Classes Require Import
      RelationClasses Morphisms.
 
 Require Import Coq.Lists.List.
+Require Import Coq.Lists.List.
 Require Import Coq.Strings.String.
 
 From ChargeCore.Logics Require Import
      ILogic BILogic ILEmbed Later.
 
 Require Import Cpp.Ast.
+Require Cpp.Parser.
 
-Require Import Coq.ZArith.BinIntDef.
+Require Import Coq.ZArith.BinInt.
+Require Import Coq.micromega.Lia.
 
 From auto.Tactics Require Import Discharge.
+
+
 
 Fixpoint arrowFrom {t} u (ls : list t) (T : Type)
 : Type :=
@@ -20,12 +25,67 @@ Fixpoint arrowFrom {t} u (ls : list t) (T : Type)
   | cons l ls => u -> arrowFrom u ls T
   end.
 
-Fixpoint forallEach {t u T} (ls : list t)
-: forall (v : arrowFrom u ls T) (P : T -> list (t * u) -> Prop), Prop :=
-  match ls with
-  | nil => fun v P => P v nil
-  | l :: ls => fun v P => forall x, forallEach ls (v x) (fun z xs => P z (cons (l, x) xs))
-  end.
+Section zip.
+  Context {A B C : Type} (f : A -> B -> C).
+  Fixpoint zip (x : list A) (y : list B) : list C :=
+    match x , y with
+    | nil , _
+    | _ , nil => nil
+    | x :: xs , y :: ys => f x y :: zip xs ys
+    end.
+End zip.
+
+
+Section withLogic.
+  Context {L : Type}.
+  Context {ILogicOps_L : ILogicOps L}.
+  Existing Instance ILogicOps_L.
+  (* Context {ILogic_L : ILogic L}. *)
+  (* Existing Instance ILogic_L. *)
+
+
+  Fixpoint applyEach {t u T} (ls : list t) (vals : list u)
+    : forall (v : arrowFrom u ls T)
+        (P : T -> list (t * u) -> L), L :=
+    match ls , vals with
+    | nil , nil => fun v P => P v nil
+    | l :: ls , x :: xs => fun v P =>
+      applyEach ls xs (v x) (fun z xs => P z (cons (l, x) xs))
+    | _ , _ => fun _ _ => lfalse
+    end.
+
+  Fixpoint ForallEach {t u T} (ls : list t)
+    : forall (v : arrowFrom u ls T)
+        (P : T -> list (t * u) -> L), L :=
+    match ls with
+    | nil => fun v P => P v nil
+    | l :: ls => fun v P => Forall x,
+      ForallEach ls (v x) (fun z xs => P z (cons (l, x) xs))
+    end.
+
+  Fixpoint Forall2Each {t u T U} (ls : list t)
+    : forall (v : arrowFrom u ls T) (v' : arrowFrom u ls U)
+        (P : T -> U -> list (t * u) -> L), L :=
+    match ls with
+    | nil => fun v v' P => P v v' nil
+    | l :: ls => fun v v' P => Forall x,
+      Forall2Each ls (v x) (v' x) (fun z z' xs => P z z' (cons (l, x) xs))
+    end.
+
+  Fixpoint ExistsEach {t u T} (ls : list t)
+    : forall (v : arrowFrom u ls T)
+        (P : T -> list (t * u) -> L), L :=
+    match ls with
+    | nil => fun v P => P v nil
+    | l :: ls => fun v P => Exists x,
+      ExistsEach ls (v x) (fun z xs => P z (cons (l, x) xs))
+    end.
+
+End withLogic.
+
+Definition forallEach := @ForallEach Prop _.
+Arguments forallEach {_ _ _}.
+
 
 Module Type logic.
 
@@ -83,6 +143,7 @@ Module Type logic.
   Parameter code_at : ptr -> Func -> mpred.
   (* code_at is freely duplicable *)
   Axiom code_at_dup : forall p f, code_at p f -|- code_at p f ** code_at p f.
+  Axiom code_at_drop : forall p f, code_at p f |-- empSP.
 
   (* it might be more uniform to have this be an `mpred` *)
   Parameter glob_addr : genv -> globname -> ptr -> Prop.
@@ -97,19 +158,6 @@ Module Type logic.
   Axiom with_genv_single : forall f g,
       with_genv f //\\ with_genv g -|- with_genv (fun r => f r //\\ g r).
 
-  Parameter func_ok_raw : Func -> list val -> (val -> mpred) -> mpred.
-  (* this assserts the frame axiom for function specifications
-   *)
-  Axiom func_ok_frame : forall v vs Q F,
-      func_ok_raw v vs Q ** F |-- func_ok_raw v vs (fun res => Q res ** F).
-
-  Definition fspec (n : val) (ls : list val) (Q : val -> mpred) : mpred :=
-    Exists f, [| n = Vptr f |] **
-    Exists func, code_at f func ** func_ok_raw func ls Q.
-
-
-  Definition function_spec (ret : type) (targs : list type) : Type :=
-    arrowFrom val targs ((val -> mpred) -> mpred).
 
   (* this is the denotation of modules *)
   Fixpoint sepSPs (ls : list mpred) : mpred :=
@@ -143,7 +191,7 @@ Module Type logic.
       with_genv (fun resolve => [| glob_addr resolve n a |]) //\\
                 code_at a f
     | Dstruct _ _ => empSP
-      (* ^ this should really record size and offset information
+      (* ^ this should record size and offset information
        *)
     | Denum _ _ _ => empSP
       (* ^ this should record enumeration information
@@ -156,11 +204,41 @@ Module Type logic.
       sepSPs (map (denoteDecl ns) ds)
     end.
 
+  Fixpoint denoteModule (ns : list ident) (d : list Decl) : mpred :=
+    match d with
+    | nil => empSP
+    | d :: ds => denoteDecl ns d ** denoteModule ns ds
+    end.
+
+  Inductive module_declares : list Decl -> globname -> Func -> Prop :=.
+
+  Axiom todo : forall t, t.
+
+  Parameter func_ok_raw : Func -> list val -> (val -> mpred) -> mpred.
+  (* this assserts the frame axiom for function specifications
+   *)
+  Axiom func_ok_frame : forall v vs Q F,
+      func_ok_raw v vs Q ** F |-- func_ok_raw v vs (fun res => Q res ** F).
+
+  Definition fspec (n : val) (ls : list val) (Q : val -> mpred) : mpred :=
+    Exists f, [| n = Vptr f |] **
+    Exists func, code_at f func ** func_ok_raw func ls Q.
+
+  (* todo(gmm): this is because func_ok is implemented using wp. *)
+  Axiom fspec_conseq:
+    forall (p : val) (vs : list val) (K m : val -> mpred),
+      (forall r : val, m r |-- K r) -> fspec p vs m |-- fspec p vs K.
+
+
+
   (** Weakest pre-condition for expressions
    *)
   Variant mode : Set := Lvalue | Rvalue.
 
-  (* todo(gmm): `wpe` should be indexed by types *)
+  (* todo(gmm): `wpe` should be indexed by types
+   * question(gmm): are lvalues just references? or is there something
+   * else to it?
+   *)
   Parameter wpe
   : forall (resolve : genv), mode -> Expr -> (val -> mpred) -> mpred.
 
@@ -264,8 +342,6 @@ Module Type logic.
         wpe resolve m e Q
         |-- wpe resolve m (Ecast Cint2bool e) Q.
 
-    Axiom wp_rhs_cast : True.
-
     Axiom wp_rhs_seqand : forall e1 e2 Q,
         wp_rhs e1 (fun v1 =>
            if is_true v1
@@ -351,13 +427,17 @@ Module Type logic.
     Definition El2r := Ecast Cl2r.
 
     Parameter has_type_int : forall z,
-        (Z.gtb z (-10000)%Z && Z.gtb (10000)%Z z = true)%bool ->
+        (-Z.pow 2 31 < z < Z.pow 2 31 - 1)%Z ->
+        has_type z T_int.
+    Parameter has_type_int32 : forall z,
+        (-Z.pow 2 31 < z < Z.pow 2 31 - 1)%Z ->
         has_type z T_int32.
     Parameter has_type_qual : forall v q ty,
         has_type v ty -> has_type v (Tqualified q ty).
 
     Ltac has_type :=
-      first [ eapply has_type_int ; reflexivity
+      first [ eapply has_type_int ; lia
+            | eapply has_type_int32 ; lia
             | eapply has_type_qual ; has_type ].
 
     Lemma eval_add : forall ty (a b c : Z),
@@ -367,11 +447,14 @@ Module Type logic.
     Admitted.
 
     Ltac operator :=
-      first [ eapply eval_add; [ reflexivity | has_type ] ].
+      first [ subst ; eapply eval_add; [ first [ reflexivity | nia ] | has_type ] ].
 
     Ltac t :=
-      let tac := try solve [ eauto | has_type | operator ] in
-      discharge tac.
+      let tac := try match goal with
+            | |- @eq val _ _ => try f_equal
+            end ;
+        try solve [ eauto | reflexivity | has_type | operator | lia ] in
+      discharge ltac:(canceler fail tac) tac.
 
     (* int x ; x = 0 ; *)
     Goal (tlocal T_int32 _x 3
@@ -564,11 +647,12 @@ Module Type logic.
         wp_decl x ty init (wp resolve (Sdecl ds)) Q
         |-- wp resolve (Sdecl ((x,ty,init) :: ds)) Q.
 
-    Require Import Cpp.Parser.
+    Import Cpp.Parser.
     Import ListNotations.
 
     Ltac simplify_wps :=
       repeat first [ progress simplify_wp
+                   | progress simpl wps
                    | rewrite <- wp_skip
                    | rewrite <- wp_seq_nil
                    | rewrite <- wp_seq_cons
@@ -588,43 +672,438 @@ Module Type logic.
     { P } - { Q } = [] (P -* wp code Q)
 *)
 
-    Fixpoint ForallEach {t u T U} (ls : list t)
-    : forall (v : arrowFrom u ls T) (v' : arrowFrom u ls U)
-        (P : T -> U -> list (t * u) -> mpred), mpred :=
-      match ls with
-      | nil => fun v v' P => P v v' nil
-      | l :: ls => fun v v' P => Forall x,
-                            ForallEach ls (v x) (v' x) (fun z z' xs => P z z' (cons (l, x) xs))
-      end.
+
+    Record function_spec' : Type :=
+    { fs'_return : type
+    ; fs'_arguments : list type
+    ; fs'_specification : arrowFrom val fs'_arguments ((val -> mpred) -> mpred)
+    }.
+
+    Record function_spec : Type :=
+    { fs_return : type
+    ; fs_arguments : list type
+    ; fs_specification : list val -> (val -> mpred) -> mpred
+    }.
+
+    Definition cptr' (p : val) (fs : function_spec') : mpred.
+    refine (ForallEach _ fs.(fs'_specification) (fun PQ args =>
+              Forall Q, PQ Q -* fspec p (List.map snd args) Q)).
+    Defined.
+
+    Definition cptr (p : val) (PQ : function_spec) : mpred.
+      refine (
+          Forall vs,
+          [| List.length vs = List.length PQ.(fs_arguments) |] -*
+          Forall Q, PQ.(fs_specification) vs Q -* fspec p vs Q).
+    Defined.
+
+    Lemma wandSP_only_provableL : forall (P : Prop) Q R,
+        P ->
+        Q |-- R ->
+        [| P |] -* Q |-- R.
+    Proof.
+      intros.
+      rewrite <- H0; clear H0.
+      etransitivity.
+      2: eapply sepSPAdj.
+      2: reflexivity.
+      rewrite <- empSPR at 1.
+      eapply scME. reflexivity.
+      discharge auto auto.
+    Qed.
+
+
+    Lemma wandSP_only_provableR : forall (A : Prop) B C,
+        (A -> B |-- C) ->
+        B |-- [| A |] -* C.
+    Proof.
+      intros.
+      unfold only_provable.
+      eapply wandSPI.
+      rewrite <- embedPropExists'.
+      specialize (landexistsDL1 (fun _: A => ltrue) empSP). simpl.
+      intros. rewrite H0.
+      setoid_rewrite landtrueL.
+      rewrite <- bilexistssc.
+      eapply lexistsL.
+      intros.
+      etransitivity; [ | eapply H ]; auto.
+      discharge fail auto.
+    Qed.
+
+    Lemma forallEach_primes:
+      forall (ts : list type)
+        (fs' : arrowFrom val ts ((val -> mpred) -> mpred)) Z,
+        Forall vs : list val,
+      [| Datatypes.length vs = Datatypes.length ts |] -*
+      (Forall Q : val -> mpred,
+                  applyEach ts vs fs'
+                            (fun (k : (val -> mpred) -> mpred) (_ : list (type * val)) => k Q) -*
+                            Z vs Q) -|-
+      ForallEach ts fs'
+      (fun (PQ : (val -> mpred) -> mpred) (args : list (type * val)) =>
+         Forall Q : val -> mpred, PQ Q -* Z (map snd args) Q).
+    Proof.
+      induction ts.
+      { simpl. intros.
+        split.
+        { eapply lforallR; intro Q.
+          eapply (lforallL nil).
+          eapply wandSP_only_provableL; [ reflexivity | ].
+          eapply lforallL. reflexivity. }
+        { eapply lforallR. intros.
+          destruct x.
+          { eapply wandSP_only_provableR. reflexivity. }
+          { eapply wandSP_only_provableR. intros.
+            inversion H. } } }
+      { simpl. intros.
+        split.
+        { eapply lforallR.
+          intros.
+          rewrite <- (IHts (fs' x) (fun a b => Z (x :: a) b)).
+          eapply lforallR. intros.
+          eapply (lforallL (x :: x0)).
+          eapply wandSP_only_provableR; intros.
+          eapply wandSP_only_provableL; [ simpl; f_equal; eassumption | ].
+          reflexivity. }
+        { eapply lforallR; intros.
+
+          eapply wandSP_only_provableR; intros.
+          destruct x.
+          { eapply lforallR; intro.
+            eapply wandSPAdj'.
+            rewrite sepSP_falseL.
+            eapply lfalseL. }
+          { eapply (lforallL v).
+            destruct (IHts (fs' v) (fun xs => Z (v :: xs))).
+            rewrite H1; clear H0 H1.
+            eapply (lforallL x).
+            eapply wandSP_only_provableL.
+            simpl in H.
+            inversion H. reflexivity. reflexivity. } } }
+    Qed.
+
+
+    Lemma cptr_cptr' : forall p fs fs',
+        fs.(fs_arguments) = fs'.(fs'_arguments) ->
+        fs.(fs_return) = fs'.(fs'_return) ->
+        (forall Q vs,
+            fs.(fs_specification) vs Q -|- applyEach fs'.(fs'_arguments) vs fs'.(fs'_specification) (fun k _ => k Q)) ->
+        cptr p fs -|- cptr' p fs'.
+    Proof.
+      unfold cptr. intros.
+      destruct fs, fs'. simpl in *. subst.
+      setoid_rewrite H1; clear H1.
+      unfold cptr'.
+      rewrite <- forallEach_primes. reflexivity.
+    Qed.
+
+
+    Record WithPrePost : Type :=
+    { wpp_with : Type
+    ; wpp_pre  : wpp_with -> mpred
+    ; wpp_post : wpp_with -> val -> mpred
+    }.
+
+    Definition ht (ret : type) (targs : list type)
+               (PQ : list val -> WithPrePost)
+      : function_spec.
+      refine (
+          {| fs_return := ret
+           ; fs_arguments := targs
+           ; fs_specification := fun args Q =>
+                Exists g : (PQ args).(wpp_with),
+                           (Forall res, (PQ args).(wpp_post) g res -* Q res)
+                             ** (PQ args).(wpp_pre) g |}).
+    Defined.
+
+    Definition ht' (ret : type) (targs : list type)
+               (PQ : arrowFrom val targs WithPrePost)
+      : function_spec'.
+    refine {| fs'_return := ret
+            ; fs'_arguments := targs
+            ; fs'_specification := _ |}.
+      induction targs.
+      { simpl in *.
+        refine (fun Q =>
+                  Exists g : PQ.(wpp_with),
+                             (Forall res, PQ.(wpp_post) g res -* Q res)
+                               ** PQ.(wpp_pre) g). }
+      { simpl in *.
+        refine (fun x => IHtargs (PQ x)). }
+    Defined.
 
 
 
-    Require Import Coq.Lists.List.
+    Theorem triple_sound : forall p r ts PQ vs,
+        List.length vs = List.length ts ->
+        forall g : (PQ vs).(wpp_with),
+          cptr p (ht r ts PQ) ** (PQ vs).(wpp_pre) g
+          |-- fspec p vs ((PQ vs).(wpp_post) g).
+    Proof.
+      unfold ht, cptr.
+      intros.
+      eapply sepSPAdj.
+      eapply (lforallL vs).
+      simpl.
+      eapply wandSP_only_provableL. auto.
+      eapply (lforallL (wpp_post (PQ vs) g)).
+      eapply wandSP_lentails_m; try reflexivity.
+      red.
+      discharge ltac:(canceler fail auto) auto.
+    Qed.
 
-    Section zip.
-      Context {A B C : Type} (f : A -> B -> C).
-      Fixpoint zip (x : list A) (y : list B) : list C :=
-        match x , y with
-        | nil , _
-        | _ , nil => nil
-        | x :: xs , y :: ys => f x y :: zip xs ys
-        end.
-    End zip.
+    Theorem triple_apply : forall p r ts F F' vs (PQ : list val -> WithPrePost) K,
+        List.length vs = List.length ts -> (* trivial *)
+        forall g : (PQ vs).(wpp_with), (* existential quantifier *)
+          F |-- (PQ vs).(wpp_pre) g ** F' -> (* pre-condition *)
+          (forall r, (PQ vs).(wpp_post) g r |-- K r) ->
+          cptr p (ht r ts PQ) ** F |-- fspec p vs K ** F'.
+    Proof.
+      intros.
+      specialize (triple_sound p r ts PQ vs H).
+      unfold ht in *.
+      rewrite H0 in *; clear H0.
+      intros.
+      specialize (H0 g).
+      rewrite <- sepSPA.
+      rewrite H0.
+      discharge ltac:(canceler fail auto) auto.
+      eapply fspec_conseq. assumption.
+    Qed.
+
+    Theorem triple'_apply
+    : forall p r ts F F' vs (PQ : arrowFrom val ts WithPrePost) K,
+        F |-- applyEach ts vs PQ (fun wpp _ =>
+                 Exists g : wpp.(wpp_with),
+                 wpp.(wpp_pre) g ** F' **
+                 (Forall r, wpp.(wpp_post) g r -* K r)) ->
+        cptr' p (ht' r ts PQ) ** F |-- fspec p vs K ** F'.
+    Proof.
+      intros.
+      rewrite <- cptr_cptr'.
+      instantiate (1:= {| fs_return := r
+                         ; fs_arguments := ts
+                         ; fs_specification := fun vs0 Q => applyEach ts vs0 (ht' r ts PQ).(fs'_specification)
+                                            (fun (k : (val -> mpred) -> mpred) (_ : list (type * val)) => k Q) |}).
+      2: intros; reflexivity.
+    Admitted.
 
     Definition func_ok (ret : type) (params : list (ident * type))
                (body : Stmt)
-               (spec : function_spec ret (map snd params))
-    : Prop.
-      red in spec.
-      eapply forallEach. eapply spec.
-      refine (fun P args => forall Q : val -> mpred,
-                  (* this is what is created from the parameters *)
-                  let binds := sepSPs (zip (fun '(x, t) '(_, v) => tlocal t x v) params args) in
-                  (* this is what is freed on return *)
-                  let frees := sepSPs (map (fun '(x, t) => Exists v, tlocal t x v) params) in
-                  (binds ** P Q) |-- (wp resolve body (Kfree frees (val_return Q)))
-             ).
+               (spec : function_spec)
+    : mpred :=
+      [| ret = spec.(fs_return) |] **
+      [| List.map snd params = spec.(fs_arguments) |] **
+      Forall args, Forall Q : val -> mpred,
+        (* this is what is created from the parameters *)
+        let binds := sepSPs (zip (fun '(x, t) 'v => tlocal t x v) params args) in
+        (* this is what is freed on return *)
+        let frees := sepSPs (map (fun '(x, t) => Exists v, tlocal t x v) params) in
+        (binds ** spec.(fs_specification) args Q) -* (wp resolve body (Kfree frees (val_return Q))).
+
+    Fixpoint ForallEach' {t u T} (ls : list t)
+    : forall (v : arrowFrom u ls T)
+        (P : T ->  list (t * u) -> mpred), mpred :=
+      match ls with
+      | nil => fun v P => P v nil
+      | l :: ls => fun v P => Forall x,
+                            ForallEach' ls (v x) (fun z xs => P z (cons (l, x) xs))
+      end.
+
+    Definition func_ok' (ret : type) (params : list (ident * type))
+               (body : Stmt)
+               (spec : function_spec')
+    : mpred.
+    refine (
+      [| ret = spec.(fs'_return) |] **
+      [| spec.(fs'_arguments) = List.map snd params |] **
+      ForallEach' _ spec.(fs'_specification) (fun PQ args =>
+        let vals := List.map snd args in
+
+        (* this is what is created from the parameters *)
+        let binds := sepSPs (zip (fun '(x, t) 'v => tlocal t x v) params vals) in
+        (* this is what is freed on return *)
+        let frees := sepSPs (map (fun '(x, t) => Exists v, tlocal t x v) params) in
+        Forall Q : val -> mpred,
+        (binds ** PQ Q) -* (wp resolve body (Kfree frees (val_return Q))))
+      ).
+    Defined.
+
+    Definition A__bar := {| g_path := "A" !:: NStop; g_name := "bar" |}.
+(*
+    Goal
+           (Exists abara, [| glob_addr resolve A__bar abara |] **
+            (cptr' (Vptr abara) T_int32 (T_int32 :: nil)
+                    (ht' T_int32 (T_int32 :: nil)
+                     (fun x => {| wpp_with := _
+                              ; wpp_pre v := [| x = Vint v |]
+                              ; wpp_post v res := [| res = Vint (Z.add v 1) |] |}))))
+        ** local "x" 3%Z
+      |-- wp resolve (Sseq [
+                (Sreturn (Some
+                  (Ebinop Badd
+                    (Ecall
+                      (Ecast Cfunction2pointer
+                        (Evar
+                          (Gname A__bar))) [
+                        (Ebinop Badd
+                          (Ecast Cl2r
+                            (Evar
+                              (Lname  "x")))
+                          (Eint 5
+                            (Qmut T_int32)))])
+                    (Eint 1
+                      (Qmut T_int32)))))])
+      (val_return (fun val => local "x" 3%Z ** [| val = Vint 10%Z |])).
+    Proof.
+      intros.
+      unfold local.
+      repeat (t; simplify_wps).
+
+      t. subst.  simplify_wps.
+      t.
     Qed.
+*)
+
+    Definition cglob' (gn : globname) (spec : function_spec')
+    : mpred :=
+      Exists a, [| glob_addr resolve gn a |] ** cptr' (Vptr a) spec.
+
+    Axiom wpe_frame : forall resolve m e k F,
+        wpe m resolve e k ** F -|- wpe m resolve e (fun x => k x ** F).
+
+    Axiom Proper_wpe_equiv
+    : Proper (eq ==> eq ==> eq ==> pointwise_relation _ lequiv ==> lequiv) wpe.
+    Axiom Proper_wpe_entails
+    : Proper (eq ==> eq ==> eq ==> pointwise_relation _ lentails ==> lentails) wpe.
+
+    Lemma wps_frame : forall es k F,
+        wps es k ** F -|- wps es (fun x => k x ** F).
+    Proof.
+      induction es; simpl; intros.
+      { reflexivity. }
+      { unfold wp_rhs. rewrite wpe_frame.
+        eapply Proper_wpe_equiv; eauto.
+        red. intros. rewrite IHes. reflexivity. }
+    Qed.
+
+    Lemma Proper_wps_entails
+    : Proper (eq ==> pointwise_relation _ lentails ==> lentails)
+             wps.
+    Proof.
+      do 3 red. intros. subst.
+      generalize dependent x0; revert y0.
+      induction y; simpl; intros.
+      { eapply H0. }
+      { simpl. eapply Proper_wpe_entails; eauto.
+        red. intros.
+        eapply IHy. red.
+        eauto. }
+    Qed.
+
+    Theorem wp_call_glob : forall f ret ts es K PQ F F',
+        F (* ** cglob' f ret ts (ht' ret ts PQ) *)
+        |-- wps es (fun vs => applyEach ts vs PQ (fun wpp _ =>
+                Exists g : wpp.(wpp_with),
+                  wpp.(wpp_pre) g ** F' **
+                  (Forall r, wpp.(wpp_post) g r -* K r))) ->
+        cglob' f (ht' ret ts PQ) ** F
+        |-- wp_rhs (Ecall (Ecast Cfunction2pointer (Evar (Gname f))) es) K ** F'.
+    Proof.
+(*
+      intros.
+      rewrite H; clear H.
+      rewrite <- wp_call.
+      rewrite <- wp_rhs_cast_function2pointer.
+      simplify_wp.
+      unfold cglob'.
+      discharge ltac:(canceler fail eauto) eauto.
+      rewrite wps_frame.
+      rewrite sepSPC.
+      rewrite wps_frame.
+      eapply Proper_wps_entails; eauto.
+      red. intros.
+      rewrite sepSPC.
+      etransitivity.
+      eapply triple'_apply with (vs:=a).
+      reflexivity.
+      discharge auto.
+      eapply spec_later_weaken.
+*)
+    Admitted.
+
+    Ltac simplifying :=
+      repeat first [ progress simplify_wp
+                   | progress simpl wps
+                   | rewrite <- wp_skip
+                   | rewrite <- wp_seq_nil
+                   | rewrite <- wp_seq_cons
+                   | rewrite <- wp_decl_nil
+                   | rewrite <- wp_decl_cons
+                   | rewrite <- wp_return_val
+                   | rewrite <- wp_return_void
+                   | rewrite <- wp_if
+                   | rewrite <- wp_continue
+                   | rewrite <- wp_break
+                   | rewrite <- wp_rhs_binop
+                   | rewrite <- wp_rhs_cast_function2pointer
+                   ].
+
+    Goal cglob' A__bar
+         (ht' T_int32 (T_int32 :: nil)
+              (fun x => {| wpp_with := _
+                       ; wpp_pre v := [| x = Vint v |]
+                       ; wpp_post v res := [| res = Vint (Z.add v 1) |] |}))
+         |--
+         func_ok' (Qmut T_int32)
+         [("x",(Qmut T_int32))]
+         (Sseq [
+              (Sreturn (Some
+                          (Ebinop Badd
+                                  (Ecall
+                                     (Ecast Cfunction2pointer
+                                            (Evar
+                                               (Gname {| g_path := "A" !:: NStop; g_name := "bar" |}))) [
+                                       (Ebinop Badd
+                                               (Ecast Cl2r
+                                                      (Evar
+                                                         (Lname  "x")))
+                                               (Eint 5
+                                                     (Qmut T_int)))])
+                                  (Eint 1
+                                        (Qmut T_int)))))])
+         (ht' (Qmut T_int32) (Qmut T_int32 :: nil) (fun x =>
+              {| wpp_with := Z
+               ; wpp_pre v := [| x = Vint v |] ** [| -100 < v < 100 |]%Z
+               ; wpp_post v res := [| res = Vint (Z.add v 7) |] |})).
+    Proof.
+      Opaque cglob' ht'.
+      unfold func_ok'. simpl.
+      Transparent ht'.
+      simpl. Opaque ht'.
+      simpl.
+      t. subst.
+      simplifying.
+      repeat perm_left ltac:(idtac; perm_right ltac:(idtac; eapply wp_call_glob)).  simpl.
+      simplifying.
+      unfold tlocal, tptsto.
+      t.
+      simplify_wps. t.
+      simplify_wps.
+      t.
+    Qed.
+
+  End with_resolver.
+
+End logic.
+
+Declare Module L : logic.
+
+Export L.
+
+
+
 
 (*
     Definition ht
@@ -671,103 +1150,45 @@ Module Type logic.
       refine (embed (
 *)
 
-    Definition triple (p : val) (ret : type) (targs : list type)
-    : arrowFrom val targs ((val -> mpred) -> mpred) -> mpred.
-      refine (
-          (fix rec ts (fspec : list val -> (val -> mpred) -> mpred)
-           : arrowFrom val ts ((val -> mpred) -> mpred) -> mpred :=
-             match ts as ts
-                   return arrowFrom val ts ((val -> mpred) -> mpred) -> mpred
-             with
-             | nil => fun PQ => Forall Q, PQ Q -* fspec nil Q
-             | t :: ts => fun PQ => Forall x, rec ts (fun xs => fspec (xs ++ x :: nil)%list) (PQ x)
-             end) targs (fspec p)).
-    Defined.
-
-    Theorem triple_sound : forall p r t PQ v Z,
-        triple p r (t :: nil) PQ ** PQ v Z |-- fspec p (v :: nil) Z.
-    Proof.
-      unfold triple.
-      intros.
-      rewrite sepSPC.
-      rewrite bilforallscR.
-      eapply lforallL with (x := v).
-      rewrite bilforallscR.
-      eapply lforallL with (x := Z).
-      simpl.
-      eapply sepSPAdj'.
-      reflexivity.
-    Qed.
-
-    Theorem triple_apply : forall p r t F F' PQ v Z,
-        F |-- PQ v Z ** F' ->
-        triple p r (t :: nil) PQ ** F |-- fspec p (v :: nil) Z ** F'.
-    Proof.
-      intros.
-      rewrite H.
-      rewrite <- triple_sound.
-      t.
-    Qed.
-
-    Definition A__bar := {| g_path := "A" !:: NStop; g_name := "bar" |}.
-    Goal
-           (Exists abara, [| glob_addr resolve A__bar abara |] **
-            (triple (Vptr abara) T_int32 (T_int32 :: nil)
-                    (fun x k => Exists v, [| x = Vint v |] ** (empSP -* k (Vint (Z.add v 1))))))
-        ** local "x" 3%Z
-      |-- wp resolve (Sseq [
-                (Sreturn (Some
-                  (Ebinop Badd
-                    (Ecall
-                      (Ecast Cfunction2pointer
-                        (Evar
-                          (Gname A__bar))) [
-                        (Ebinop Badd
-                          (Ecast Cl2r
-                            (Evar
-                              (Lname  "x")))
-                          (Eint 5
-                            (Qmut T_int32)))])
-                    (Eint 1
-                      (Qmut T_int32)))))])
-      (val_return (fun val => local "x" 3%Z ** [| val = Vint 10%Z |])).
-    Proof.
-      intros.
-      repeat (t; simplify_wps).
-      simpl.
-      (t; simplify_wps).
-      unfold local.
-      repeat (t; simplify_wps).
-      etransitivity; [ | eapply spec_later_weaken ].
-      repeat perm_left ltac:(idtac; perm_right ltac:(idtac; eapply triple_apply)).
-      t. simplify_wps.
-      t.
-    Qed.
-
 (*
+  Theorem triple_sound : forall p r t PQ v Z,
+      triple p r (t :: nil) PQ ** PQ v Z |-- fspec p (v :: nil) Z.
+  Proof.
+    unfold triple.
+    intros.
+    rewrite sepSPC.
+    rewrite bilforallscR.
+    eapply lforallL with (x := v).
+    rewrite bilforallscR.
+    eapply lforallL with (x := Z).
+    simpl.
+    eapply sepSPAdj'.
+    reflexivity.
+  Qed.
 
-    Goal func_ok (Qmut T_int)
-         [("x",(Qmut T_int))]
-         (Sseq [
-              (Sreturn (Some
-                          (Ebinop Badd
-                                  (Ecall
-                                     (Ecast Cfunction2pointer
-                                            (Evar
-                                               (Gname {| g_path := "A" !:: NStop; g_name := "bar" |}))) [
-                                       (Ebinop Badd
-                                               (Ecast Cl2r
-                                                      (Evar
-                                                         (Lname  "x")))
-                                               (Eint 5
-                                                     (Qmut T_int)))])
-                                  (Eint 1
-                                        (Qmut T_int)))))])
-         (fun x k => _).
-:: nil.
-
+  Theorem triple_apply : forall p r t F F' PQ v Z,
+      F |-- PQ v Z ** F' ->
+      triple p r (t :: nil) PQ ** F |-- fspec p (v :: nil) Z ** F'.
+  Proof.
+    intros.
+    rewrite H.
+    rewrite <- triple_sound.
+    discharge auto.
+  Qed.
 *)
 
-  End with_resolver.
-
-End logic.
+    (*
+  Definition func_ok (ret : type) (params : list (ident * type))
+             (body : Stmt)
+             (spec : function_spec ret (map snd params))
+  : Prop.
+    red in spec.
+    refine (forall args (Q : val -> mpred),
+      (* this is what is created from the parameters *)
+      let binds := sepSPs (zip (fun '(x, t) 'v => tlocal t x v) params args) in
+      (* this is what is freed on return *)
+      let frees := sepSPs (map (fun '(x, t) => Exists v, tlocal t x v) params) in
+      (binds ** spec args Q) |-- (wp resolve body (Kfree frees (val_return Q)))
+           ).
+  Defined.
+     *)
